Cas-wp rules from iris from the ground up.
The proofs mainly follow the structure for wpr-put. In terms of the heap
lemmas. Afterall it is simply wp-put with extra steps.

theories/program_logic/itree.v
@@ -45,6 +45,7 @@ Definition get {V} (l: loc): expr V V := Vis (GetE l) Answer.
 Definition put {V} (l: loc) (v: V): expr V () := Vis (PutE l v) Answer .
 Definition alloc {V} (v: V): expr V loc := Vis (AllocE v) Answer.
 Definition free {V} (l: loc): expr V () := Vis (FreeE l) Answer.
+Definition cas {V} (l: loc) (v1 v2: V): expr V (V * bool) := Vis (CasE l v1 v2) Answer.
 
 (* Apply the continuation k to the Ret nodes of the itree t *)
 Instance itree_bind {E}: MBind (itree E) := λ R S k, 
